SimAsm/SimAsm.thy
@@ -19,7 +19,7 @@ datatype ('r,'v,'s,'a) lang =
   | Seq "('r,'v,'s,'a) lang" "('r,'v,'s,'a) lang"
   | If "('r,'v) bexp" "('r,'v,'s,'a) lang" "('r,'v,'s,'a) lang"  
   | While "('r,'v) bexp" "('r,'v,'s,'a) pred" "('r,'v,'s,'a) pred" "('r,'v,'s,'a) lang"
-  | DoWhile "('r,'v,'s,'a) pred" "('r,'v,'s,'a) lang" "('r,'v) bexp"
+  | DoWhile "('r,'v,'s,'a) pred" "('r,'v,'s,'a) pred" "('r,'v,'s,'a) lang" "('r,'v) bexp"
 
 
 context expression
