SimAsm/SimAsm_Reasoning.thy
@@ -1,0 +1,234 @@
+theory SimAsm_Reasoning
+  imports SimAsm_WP 
+begin
+
+
+section \<open>Locales for reasoning, either with speculation (reasoning_spec) or without (reasoning_WOspec)\<close>
+
+(* We are using unlablled states from here onwards; labelling only occurs in some parts of the
+    wp reasoning *)
+
+
+(*---------------------------------------------------------------------------------------*)
+
+locale reasoning_WOspec = wp_WOspec + expression st st_upd aux aux_upd locals
+  for st :: "('r,'v,'a) varmap' \<Rightarrow> 'r \<Rightarrow> 'v"
+  and st_upd :: "('r,'v,'a) varmap' \<Rightarrow> 'r \<Rightarrow> 'v \<Rightarrow> ('r,'v,'a) varmap'"
+  and aux :: "('r,'v,'a) varmap' \<Rightarrow> 'a"
+  and aux_upd :: "('r,'v,'a) varmap' \<Rightarrow> (('r,'v,'a) varmap' \<Rightarrow> 'a) \<Rightarrow> ('r,'v,'a) varmap'"
+  and locals :: "'r set"
+
+print_locale reasoning_WOspec
+
+context reasoning_WOspec
+begin
+
+definition reorder_inst :: "('r,'v,'a) opbasic' \<Rightarrow> ('r,'v,'a) opbasic' \<Rightarrow> ('r,'v,'a) opbasic' \<Rightarrow> bool"
+  where "reorder_inst \<alpha>' \<beta> \<alpha>  \<equiv> (re\<^sub>s \<beta> \<alpha> \<and> (\<alpha>'=fwd\<^sub>s \<alpha> (fst \<beta>)))"
+
+abbreviation Seqw (infixr ";;" 80)                      (* i.e., Seq c w c' *)
+  where "Seqw c c' \<equiv> com.Seq c reorder_inst c'"
+
+abbreviation Iterw ("_*" [90] 90)                       (* i.e., Loop c w *)
+  where "Iterw c \<equiv> com.Loop c reorder_inst"
+
+text \<open>Convert the language into the abstract language expected by the underlying logic
+      this relates the syntax to its semantics \<close> 
+fun lift\<^sub>c :: "('r,'v,('r,'v,'a) varmap','a) lang \<Rightarrow> (('r,'v,'a) auxop', ('r,'v,'a) varmap') com" 
+  where
+    "lift\<^sub>c Skip = com.Nil" |
+    "lift\<^sub>c (Op v a f) = Basic (liftg v a f)" | 
+    "lift\<^sub>c (lang.Seq c\<^sub>1 c\<^sub>2) = (lift\<^sub>c c\<^sub>1) ;; (lift\<^sub>c c\<^sub>2)" |  
+    "lift\<^sub>c (If b c\<^sub>1 c\<^sub>2) = (Choice (\<lambda> s. if (st_ev\<^sub>B s b)
+                                 then (Basic (\<lfloor>cmp b\<rfloor>) ;; (lift\<^sub>c c\<^sub>1)) 
+                                 else (Basic (\<lfloor>ncmp b\<rfloor>) ;; (lift\<^sub>c c\<^sub>2))))" | 
+    "lift\<^sub>c (While b Imix Ispec c) =  (Basic (\<lfloor>cmp b\<rfloor>) ;; (lift\<^sub>c c))* ;; Basic (\<lfloor>ncmp b\<rfloor>)" | 
+    "lift\<^sub>c (DoWhile Imix Ispec c b) =  (lift\<^sub>c c ;; Basic (\<lfloor>cmp b\<rfloor>))* ;; lift\<^sub>c c ;; Basic (\<lfloor>ncmp b\<rfloor>)" 
+
+text \<open>The language is always thread-local\<close>
+lemma local_lift [intro]:
+  "local (lift\<^sub>c c)"
+  by (induct c) auto
+
+
+end
+
+(*---------------------------------------------------------------------------------------*)
+
+locale reasoning_spec = wp_spec + expression st st_upd aux aux_upd locals
+  for st :: "('r,'v,'a) varmap' \<Rightarrow> 'r \<Rightarrow> 'v"
+  and st_upd :: "('r,'v,'a) varmap' \<Rightarrow> 'r \<Rightarrow> 'v \<Rightarrow> ('r,'v,'a) varmap'"
+  and aux :: "('r,'v,'a) varmap' \<Rightarrow> 'a"
+  and aux_upd :: "('r,'v,'a) varmap' \<Rightarrow> (('r,'v,'a) varmap' \<Rightarrow> 'a) \<Rightarrow> ('r,'v,'a) varmap'"
+  and locals :: "'r set"
+
+print_locale reasoning_spec
+
+
+context reasoning_spec
+begin
+
+text \<open> definition for weak memory model which is used as parameter w in sequential composition \<close>
+
+definition sc :: "('r,'v,'a) opbasic' \<Rightarrow> ('r,'v,'a) opbasic' \<Rightarrow> ('r,'v,'a) opbasic' \<Rightarrow> bool" 
+  where "sc \<alpha>' \<beta> \<alpha>  \<equiv> \<not>(re\<^sub>s \<beta> \<alpha>)"
+
+abbreviation Seqsc (infixr "." 80)                      (* i.e., Seq c sc c' *)
+  where "Seqsc c c' \<equiv> com.Seq c sc c'"
+
+abbreviation Itersc ("_**" [90] 90)                       (* i.e., Loop c sc *)
+  where "Itersc c \<equiv> com.Loop c sc"
+
+
+definition reorder_inst :: "('r,'v,'a) opbasic' \<Rightarrow> ('r,'v,'a) opbasic' \<Rightarrow> ('r,'v,'a) opbasic' \<Rightarrow> bool"
+  where "reorder_inst \<alpha>' \<beta> \<alpha>  \<equiv> (re\<^sub>s \<beta> \<alpha> \<and> (\<alpha>'=fwd\<^sub>s \<alpha> (fst \<beta>)))"
+
+abbreviation Seqw (infixr ";;" 80)                      (* i.e., Seq c w c' *)
+  where "Seqw c c' \<equiv> com.Seq c reorder_inst c'"
+
+abbreviation Iterw ("_*" [90] 90)                       (* i.e., Loop c w *)
+  where "Iterw c \<equiv> com.Loop c reorder_inst"
+
+
+
+text \<open>Convert the language into the abstract language expected by the underlying logic
+      this relates the syntax to its semantics 
+      The conversion carries a command as a second parameter around, which models the "lifted rest", 
+       to allow for modelling the speculation of unlimited speculation frames 
+       (i.e, speculates over the rest r of the program).
+      The "rest" is relative within composed language constructs (e.g., in Seq c1 c2 rest of c1 
+       differs from rest of c2) \<close> 
+
+
+function lift\<^sub>c :: "('r,'v,('r,'v,'a) varmap','a) lang \<Rightarrow> (('r,'v,'a) auxop', ('r,'v,'a) varmap') com \<Rightarrow> 
+                                                       (('r,'v,'a) auxop', ('r,'v,'a) varmap') com" 
+  where
+    "lift\<^sub>c Skip r = com.Nil" |
+    "lift\<^sub>c (Op v a f) r = Basic (\<lfloor>v,a,f\<rfloor>)" | 
+    "lift\<^sub>c (Seq c\<^sub>1 c\<^sub>2) r = (lift\<^sub>c c\<^sub>1 (lift\<^sub>c c\<^sub>2 r)) ;; (lift\<^sub>c c\<^sub>2 r)" |  
+    "lift\<^sub>c (If b c\<^sub>1 c\<^sub>2) r =  (Choice (\<lambda> s. if (st_ev\<^sub>B s b)
+                    then Interrupt (\<forall>\<^sub>c((lift\<^sub>c  c\<^sub>2 r) ;; r)) . (Basic (\<lfloor>cmp b\<rfloor>) ;; (lift\<^sub>c c\<^sub>1 r)) 
+                    else Interrupt (\<forall>\<^sub>c((lift\<^sub>c c\<^sub>1 r) ;; r)) . (Basic (\<lfloor>ncmp b\<rfloor>) ;; (lift\<^sub>c c\<^sub>2 r))))" |
+    "lift\<^sub>c (While b Imix Ispec c) r = (Choice (\<lambda> s. if (st_ev\<^sub>B s b)
+                    then Interrupt (\<forall>\<^sub>c(r)) . (Basic (\<lfloor>cmp b\<rfloor>) ;; (lift\<^sub>c c r)) 
+                    else Interrupt (\<forall>\<^sub>c((lift\<^sub>c c r) ;; r)) . (Basic (\<lfloor>ncmp b\<rfloor>))))" |
+    "lift\<^sub>c (DoWhile Imix Ispec c b) r = ((lift\<^sub>c c (Basic (\<lfloor>cmp b\<rfloor>) ;; r)) ;; Basic (\<lfloor>cmp b\<rfloor>))* ;; 
+                                         (lift\<^sub>c c (Basic (\<lfloor>ncmp b\<rfloor>) ;; r)) ;; Basic (\<lfloor>ncmp b\<rfloor>)" 
+
+  apply pat_completeness by auto 
+
+
+
+text \<open>The language is always thread-local\<close>
+lemma local_lift [intro]:
+  "local (lift\<^sub>c c r)"
+  apply (induct c) 
+  sorry
+
+end   (* end of reasoning_spec *)
+
+(*---------------------------------------------------------------------------------------*)
+
+print_locale reasoning_spec
+
+text \<open> The locale reasoning is currently set to reasoning with speculation 
+        but it can be set to reasoning without speculation by replacing 
+        reasoning_spec --> reasoning_WOspec \<close>
+
+
+locale reasoning = reasoning_spec project rg glb st st_upd aux aux_upd locals
+  for project :: "('b \<Rightarrow> 'c) \<Rightarrow> ('b, 'c, 'd) varmap_rec_scheme"
+  and rg :: "('b, 'c, 'd) varmap_rec_scheme \<Rightarrow> 'e"
+  and glb :: "('b, 'c, 'd) varmap_rec_scheme \<Rightarrow> 'f"
+  and st :: "('r,'v,'a) varmap' \<Rightarrow> 'r \<Rightarrow> 'v"
+  and st_upd :: "('r,'v,'a) varmap' \<Rightarrow> 'r \<Rightarrow> 'v \<Rightarrow> ('r,'v,'a) varmap'"
+  and aux :: "('r,'v,'a) varmap' \<Rightarrow> 'a"
+  and aux_upd :: "('r,'v,'a) varmap' \<Rightarrow> (('r,'v,'a) varmap' \<Rightarrow> 'a) \<Rightarrow> ('r,'v,'a) varmap'"
+  and locals :: "'r set"
+
+print_locale reasoning
+
+context reasoning
+begin
+
+(* TODO:
+  in lift\<^sub>c we have to model how lang maps to its semantics;
+  to model speculative execution, we have to match
+      lift\<^sub>c (While b I c) = ...
+      lift\<^sub>c (DoWhile I c b) = 
+*)
+
+(* these two dummy parameters used in the interpretation of locale rules, locale semantics resp.,
+    and help to instantiate the types of auxop and state*)
+
+abbreviation "someAuxOp ::('v,'g,'r,'a) auxop  \<equiv> undefined"
+abbreviation "someState ::('r \<Rightarrow> 'v) \<equiv> undefined" (* add a push instance *)
+
+print_locale rules 
+
+interpretation rules  (* No type arity state_rec_ext :: pstate  when "someAuxOp" "someState" *)
+  done
+
+term obs 
+term lexecute
+term lift\<^sub>c 
+print_locale rules
+
+
+
+text \<open>Extract the instruction from an abstract operation \<close>
+(* tag (opbasic) = (op \<times> auxfn) *)
+abbreviation inst :: "('r,'v,'a) opbasic' \<Rightarrow> ('r,'v) op"
+  where "inst a \<equiv> fst (tag a)"
+
+abbreviation auxbasic :: "('r,'v,('r,'v,'a) varmap','a) opbasic \<Rightarrow> (('r,'v,'a) varmap','a) auxfn"
+  where "auxbasic a \<equiv> snd (tag a)"
+
+text \<open>A basic is well-formed if its behaviour (i.e., its abstract semantics) agrees with the behaviour
+      of its instruction and auxiliary composed (i.e., the concrete semantics of the instantiation).\<close>
+(* beh \<beta> = snd (snd \<beta>) *)
+definition wfbasic :: "('r,'v,'a) opbasic' \<Rightarrow> bool"
+  where "wfbasic \<beta> \<equiv> beh \<beta> = beh\<^sub>a (inst \<beta>, auxbasic \<beta>)"
+
+
+lemma opbasicE:
+    obtains (assign) x e f v b where  "(basic ) = ((assign x e,f), v, b)" |
+          (cmp) g f v b where "(basic ) = ((cmp g,f), v, b)" |
+          (fence) f v b where "(basic ) = ((full_fence,f), v, b)" |
+          (nop) f v b where "(basic ) = ((nop,f), v, b)" |
+          (leak) c e f v b where "(basic ) = ((leak c e,f), v, b)" 
+  by (cases basic, case_tac a, case_tac aa; clarsimp) 
+
+lemma [simp]:
+  "wr (inst (fwd\<^sub>s \<alpha> (tag \<beta>))) = wr (inst \<alpha>)"
+  by (cases \<alpha> rule: opbasicE; cases \<beta> rule: opbasicE; auto simp: Let_def split: if_splits)
+
+lemma [simp]:
+  "barriers (inst (fwd\<^sub>s \<alpha> (tag \<beta>))) = barriers (inst \<alpha>)"
+  by (cases \<alpha> rule: opbasicE; cases \<beta> rule: opbasicE; auto simp: Let_def split: if_splits)
+
+lemma [simp]:
+"rd (inst (fwd\<^sub>s \<alpha> (tag \<beta>))) = (if wr (inst \<beta>) \<inter> rd (inst \<alpha>) \<noteq> {} 
+                                  then rd (inst \<alpha>) - wr (inst \<beta>) \<union> rd (inst \<beta>) else rd (inst \<alpha>))"
+  by (cases \<alpha> rule: opbasicE; cases \<beta> rule: opbasicE; auto)
+
+lemma vc_fwd\<^sub>s[simp]:
+  "vc (fwd\<^sub>s \<alpha> \<beta>) = vc \<alpha>"
+  by (cases \<alpha> rule: opbasicE; cases \<beta>; case_tac a; auto simp: Let_def split: if_splits)
+
+lemma beh_fwd\<^sub>s [simp]:
+  "beh (fwd\<^sub>s \<alpha> \<beta>) = ( beh\<^sub>a (fwd\<^sub>i (inst \<alpha>) (fst \<beta>), (auxbasic \<alpha>)) )"
+  by (cases \<alpha> rule: opbasicE; cases \<beta>; case_tac a; auto simp: wfbasic_def Let_def split: if_splits) 
+
+lemma aux_fwd\<^sub>s [simp]:
+  "auxbasic (fwd\<^sub>s \<alpha> \<beta>) = auxbasic \<alpha>"
+  by (cases \<alpha> rule: opbasicE; cases \<beta>; case_tac a; auto simp: Let_def split: if_splits)
+
+lemma inst_fwd\<^sub>s [simp]:
+  "inst (fwd\<^sub>s \<alpha> (assign x e, f)) = subst\<^sub>i (inst \<alpha>) x e"
+  by (cases \<alpha> rule: opbasicE; auto simp: Let_def split: if_splits)
+
+
+end  (* end of context reasoning *)
+
+end
